chapter05-dsm/exercises/exercise02.dfy
@@ -1,0 +1,64 @@
+//#title Two Phase Commit Safety Specification Predicate
+//#desc Express the English Atomic Commit safety properties as predicates
+//#desc over the compound state machine model from exercise01.
+
+/*
+ * 2PC should satisfy the Atomic Commit specification. English design doc:
+ *
+ * AC-1: All processes that reach a decision reach the same one.
+ * AC-3: The Commit decision can only be reached if all processes prefer Yes.
+ * AC-4: If all processes prefer Yes, then the decision must be Commit.
+ *
+ * Note that the full Atomic Commit spec includes these additional properties,
+ * but you should ignore them for this exercise:
+ * AC-2: (stability) A process cannot reverse its decision after it has reached one.
+ *       (best modeled with refinement)
+ * AC-5: (liveness) All processes eventually decide.
+ *
+ */
+
+// Note that we include the result of exercise01. If you have doubts about the
+// model you built there, please contact an instructor for a correct solution
+// to build on for this exercise.
+include "exercise01.dfy"
+
+module Obligations {
+  import opened Types
+  import opened Library
+  import opened DistributedSystem
+
+  // AC-1: All processes that reach a decision reach the same one.
+  predicate SafetyAC1(c: Constants, v: Variables)
+    requires Host.GroupWF(c.hosts, v.hosts)
+  {
+    // All hosts that reach a decision reach the same one
+    true
+  }
+
+  // AC2 is sort of a history predicate; we're going to ignore it.
+
+  // AC-3: The Commit decision can only be reached if all processes prefer Yes.
+  predicate SafetyAC3(c: Constants, v: Variables)
+    requires Host.GroupWF(c.hosts, v.hosts)
+  {
+    true
+  }
+
+  // AC-4: If all processes prefer Yes, then the decision must be Commit.
+  predicate SafetyAC4(c: Constants, v: Variables)
+    requires Host.GroupWF(c.hosts, v.hosts)
+  {
+    true
+  }
+
+  // AC5 is a liveness proprety, we're definitely going to ignore it.
+
+  //#instructor Player 1
+  predicate Safety(c: Constants, v: Variables)
+    requires Host.GroupWF(c.hosts, v.hosts)
+  {
+    && SafetyAC1(c, v)
+    && SafetyAC3(c, v)
+    && SafetyAC4(c, v)
+  }
+}
