chapter05-dsm/exercises/exercise03.dfy
@@ -1,0 +1,98 @@
+//#title Two Phase Commit Safety Proof
+//#desc Model a distributed protocol using compound state machines.
+
+// TODO(manos): how should we ensure this file is disseminated at the
+// appropriate time, so students aren't waiting for it?
+//
+// Please begin with a copy of the official solution to exercises 01 & 02,
+// to ensure you're not doing battle with mistakes in your own protocol definition.
+// The proof is challenging enough for an exercise without fighting protocol bugs.
+include "exercise02-solution.dfy"
+
+module Proof {
+  import opened Types
+  import opened Library
+  import opened DistributedSystem
+  import opened Obligations
+
+  predicate VoteMessagesAgreeWithParticipantPreferences(c: Constants, v: Variables)
+    requires Host.GroupWF(c.hosts, v.hosts)
+  {
+    (forall msg |
+      && msg in v.network.sentMsgs
+      && msg.VoteMsg?
+      && ValidParticipantId(c, msg.sender)
+      :: msg.vote == ParticipantConstants(c, msg.sender).preference
+    )
+  }
+
+  predicate CoordinatorStateSupportedByVote(c: Constants, v: Variables)
+    requires Host.GroupWF(c.hosts, v.hosts)
+  {
+    (forall idx:HostId |
+      && ValidParticipantId(c, idx)
+      && CoordinatorVars(c, v).votes[idx].Some?
+      :: VoteMsg(idx, CoordinatorVars(c, v).votes[idx].value) in v.network.sentMsgs
+    )
+  }
+
+  predicate DecisionMsgsAgreeWithDecision(c: Constants, v: Variables)
+    requires Host.GroupWF(c.hosts, v.hosts)
+  {
+    (forall msg |
+      && msg in v.network.sentMsgs
+      && msg.DecisionMsg?
+      :: CoordinatorHost.ObservesResult(CoordinatorConstants(c), CoordinatorVars(c, v), msg.decision)
+    )
+  }
+
+  predicate Inv(c: Constants, v: Variables)
+  {
+    && Host.GroupWF(c.hosts, v.hosts)
+    && VoteMessagesAgreeWithParticipantPreferences(c, v)
+    && CoordinatorStateSupportedByVote(c, v)
+    && DecisionMsgsAgreeWithDecision(c, v)
+    && Safety(c, v)
+  }
+
+  lemma InitImpliesInv(c: Constants, v: Variables)
+    requires Init(c, v)
+    ensures Inv(c, v)
+  {
+    // Nobody has agreed with anything yet, so they agree with both.
+    assert AllWithDecisionAgreeWithThisOne(c, v, Commit); // witness.
+    assert AllWithDecisionAgreeWithThisOne(c, v, Abort); // witness.
+  }
+
+  lemma InvInductive(c: Constants, v: Variables, v': Variables)
+    requires Inv(c, v)
+    requires Next(c, v, v')
+    ensures Inv(c, v')
+  {
+    // The body of this lemma got really big (expanding foralls, case splits,
+    // testing asserts) while I was figuring out what invariants were missing
+    // ... and fixing a couple of errors in the protocol definition itself.
+    // Afterward, nearly all of that text could be deleted.
+
+    var step :| NextStep(c, v, v', step);   // Witness
+
+    forall msg |
+      && msg in v'.network.sentMsgs
+      && msg.VoteMsg?
+      && ValidParticipantId(c, msg.sender)
+      ensures msg.vote == ParticipantConstants(c, msg.sender).preference
+    {
+      var hostid := step.hostid;
+      assert Host.Next(c.hosts[hostid], v.hosts[hostid], v'.hosts[hostid], step.msgOps);
+    }
+    assert VoteMessagesAgreeWithParticipantPreferences(c, v');
+
+    assert Safety(c, v');
+  }
+
+  lemma InvImpliesSafety(c: Constants, v: Variables)
+    requires Inv(c, v)
+    ensures Safety(c, v)
+  { // Trivial, as usual, since safety is a conjunct in Inv.
+  }
+}
